isabelle2021-1: sync Word_Lib from afp
Signed-off-by: Gerwin Klein <gerwin.klein@proofcraft.systems>

lib/Word_Lib/Generic_set_bit.thy
@@ -11,15 +11,16 @@ section \<open>Operation variant for setting and unsetting bits\<close>
 theory Generic_set_bit
   imports
     "HOL-Library.Word"
-    Bits_Int
     Most_significant_bit
 begin
 
 class set_bit = semiring_bits +
   fixes set_bit :: \<open>'a \<Rightarrow> nat \<Rightarrow> bool \<Rightarrow> 'a\<close>
-  assumes bit_set_bit_iff [bit_simps]:
+  assumes bit_set_bit_iff_2n:
     \<open>bit (set_bit a m b) n \<longleftrightarrow>
       (if m = n then b else bit a n) \<and> 2 ^ n \<noteq> 0\<close>
+
+lemmas bit_set_bit_iff[bit_simps] = bit_set_bit_iff_2n[simplified fold_possible_bit simp_thms]
 
 lemma set_bit_eq:
   \<open>set_bit a n b = (if b then Bit_Operations.set_bit else unset_bit) n a\<close>
@@ -30,88 +31,43 @@ instantiation int :: set_bit
 begin
 
 definition set_bit_int :: \<open>int \<Rightarrow> nat \<Rightarrow> bool \<Rightarrow> int\<close>
-  where \<open>set_bit i n b = bin_sc n b i\<close>
+  where \<open>set_bit_int i n b = (if b then Bit_Operations.set_bit else Bit_Operations.unset_bit) n i\<close>
 
 instance
-  by standard
-    (simp_all add: set_bit_int_def bin_nth_sc_gen bit_simps)
+  by standard (simp_all add: set_bit_int_def bit_simps)
 
 end
-
-lemma int_set_bit_0 [simp]: fixes x :: int shows
-  "set_bit x 0 b = of_bool b + 2 * (x div 2)"
-  by (auto simp add: set_bit_int_def intro: bin_rl_eqI)
-
-lemma int_set_bit_Suc: fixes x :: int shows
-  "set_bit x (Suc n) b = of_bool (odd x) + 2 * set_bit (x div 2) n b"
-  by (auto simp add: set_bit_int_def intro: bin_rl_eqI)
-
-lemma bin_last_set_bit:
-  "bin_last (set_bit x n b) = (if n > 0 then bin_last x else b)"
-  by (cases n) (simp_all add: int_set_bit_Suc)
-
-lemma bin_rest_set_bit:
-  "bin_rest (set_bit x n b) = (if n > 0 then set_bit (x div 2) (n - 1) b else x div 2)"
-  by (cases n) (simp_all add: int_set_bit_Suc)
-
-lemma int_set_bit_numeral: fixes x :: int shows
-  "set_bit x (numeral w) b = of_bool (odd x) + 2 * set_bit (x div 2) (pred_numeral w) b"
-  by (simp add: set_bit_int_def)
-
-lemmas int_set_bit_numerals [simp] =
-  int_set_bit_numeral[where x="numeral w'"]
-  int_set_bit_numeral[where x="- numeral w'"]
-  int_set_bit_numeral[where x="Numeral1"]
-  int_set_bit_numeral[where x="1"]
-  int_set_bit_numeral[where x="0"]
-  int_set_bit_Suc[where x="numeral w'"]
-  int_set_bit_Suc[where x="- numeral w'"]
-  int_set_bit_Suc[where x="Numeral1"]
-  int_set_bit_Suc[where x="1"]
-  int_set_bit_Suc[where x="0"]
-  for w'
-
-lemma msb_set_bit [simp]: "msb (set_bit (x :: int) n b) \<longleftrightarrow> msb x"
-by(simp add: msb_conv_bin_sign set_bit_int_def)
 
 instantiation word :: (len) set_bit
 begin
 
 definition set_bit_word :: \<open>'a word \<Rightarrow> nat \<Rightarrow> bool \<Rightarrow> 'a word\<close>
-  where word_set_bit_def: \<open>set_bit a n x = word_of_int (bin_sc n x (uint a))\<close>
+  where set_bit_unfold: \<open>set_bit w n b = (if b then Bit_Operations.set_bit n w else unset_bit n w)\<close>
+  for w :: \<open>'a::len word\<close>
 
 instance
-  by standard
-    (auto simp add: word_set_bit_def bin_nth_sc_gen bit_simps)
+  by standard (auto simp add: set_bit_unfold bit_simps dest: bit_imp_le_length)
 
 end
-
-lemma set_bit_unfold:
-  \<open>set_bit w n b = (if b then Bit_Operations.set_bit n w else unset_bit n w)\<close>
-  for w :: \<open>'a::len word\<close>
-  by (simp add: set_bit_eq)
 
 lemma bit_set_bit_word_iff [bit_simps]:
   \<open>bit (set_bit w m b) n \<longleftrightarrow> (if m = n then n < LENGTH('a) \<and> b else bit w n)\<close>
   for w :: \<open>'a::len word\<close>
   by (auto simp add: bit_simps dest: bit_imp_le_length)
 
-lemma word_set_nth [simp]: "set_bit w n (test_bit w n) = w"
-  for w :: "'a::len word"
-  by (auto simp: word_test_bit_def word_set_bit_def)
-
-lemma test_bit_set: "(set_bit w n x) !! n \<longleftrightarrow> n < size w \<and> x"
-  for w :: "'a::len word"
-  by (auto simp: word_size word_test_bit_def word_set_bit_def nth_bintr)
-
 lemma test_bit_set_gen:
-  "test_bit (set_bit w n x) m = (if m = n then n < size w \<and> x else test_bit w m)"
+  "bit (set_bit w n x) m \<longleftrightarrow> (if m = n then n < size w \<and> x else bit w m)"
   for w :: "'a::len word"
-  apply (unfold word_size word_test_bit_def word_set_bit_def)
-  apply (clarsimp simp add: nth_bintr bin_nth_sc_gen)
-  apply (auto elim!: test_bit_size [unfolded word_size]
-      simp add: word_test_bit_def [symmetric])
-  done
+  by (simp add: bit_set_bit_word_iff word_size)
+
+lemma test_bit_set:
+  "bit (set_bit w n x) n \<longleftrightarrow> n < size w \<and> x"
+  for w :: "'a::len word"
+  by (auto simp add: bit_simps word_size)
+
+lemma word_set_nth: "set_bit w n (bit w n) = w"
+  for w :: "'a::len word"
+  by (rule bit_word_eqI) (simp add: bit_simps)
 
 lemma word_set_set_same [simp]: "set_bit (set_bit w n x) n y = set_bit w n y"
   for w :: "'a::len word"
@@ -123,27 +79,7 @@ lemma word_set_set_diff:
   shows "set_bit (set_bit w m x) n y = set_bit (set_bit w n y) m x"
   by (rule word_eqI) (auto simp: test_bit_set_gen word_size assms)
 
-lemma set_bit_word_of_int: "set_bit (word_of_int x) n b = word_of_int (bin_sc n b x)"
-  unfolding word_set_bit_def
-  by (rule word_eqI)(simp add: word_size bin_nth_sc_gen nth_bintr)
-
-lemma word_set_numeral [simp]:
-  "set_bit (numeral bin::'a::len word) n b =
-    word_of_int (bin_sc n b (numeral bin))"
-  unfolding word_numeral_alt by (rule set_bit_word_of_int)
-
-lemma word_set_neg_numeral [simp]:
-  "set_bit (- numeral bin::'a::len word) n b =
-    word_of_int (bin_sc n b (- numeral bin))"
-  unfolding word_neg_numeral_alt by (rule set_bit_word_of_int)
-
-lemma word_set_bit_0 [simp]: "set_bit 0 n b = word_of_int (bin_sc n b 0)"
-  unfolding word_0_wi by (rule set_bit_word_of_int)
-
-lemma word_set_bit_1 [simp]: "set_bit 1 n b = word_of_int (bin_sc n b 1)"
-  unfolding word_1_wi by (rule set_bit_word_of_int)
-
-lemma word_set_nth_iff: "set_bit w n b = w \<longleftrightarrow> w !! n = b \<or> n \<ge> size w"
+lemma word_set_nth_iff: "set_bit w n b = w \<longleftrightarrow> bit w n = b \<or> n \<ge> size w"
   for w :: "'a::len word"
   apply (rule iffI)
    apply (rule disjCI)
@@ -153,38 +89,36 @@ lemma word_set_nth_iff: "set_bit w n b = w \<longleftrightarrow> w !! n = b \<or
   apply (erule disjE)
    apply clarsimp
   apply (rule word_eqI)
-  apply (clarsimp simp add : test_bit_set_gen)
-  apply (drule test_bit_size)
-  apply force
+   apply (clarsimp simp add : test_bit_set_gen)
+   apply (auto simp add: word_size)
+  apply (rule bit_eqI)
+  apply (simp add: bit_simps)
   done
 
 lemma word_clr_le: "w \<ge> set_bit w n False"
   for w :: "'a::len word"
-  apply (simp add: word_set_bit_def word_le_def)
+  apply (simp add: set_bit_unfold)
   apply transfer
-  apply (rule order_trans)
-   apply (rule bintr_bin_clr_le)
-  apply simp
+  apply (simp add: take_bit_unset_bit_eq unset_bit_less_eq)
   done
 
 lemma word_set_ge: "w \<le> set_bit w n True"
   for w :: "'a::len word"
-  apply (simp add: word_set_bit_def word_le_def)
+  apply (simp add: set_bit_unfold)
   apply transfer
-  apply (rule order_trans [OF _ bintr_bin_set_ge])
-  apply simp
+  apply (simp add: take_bit_set_bit_eq set_bit_greater_eq)
   done
 
 lemma set_bit_beyond:
   "size x \<le> n \<Longrightarrow> set_bit x n b = x" for x :: "'a :: len word"
-  by (auto intro: word_eqI simp add: test_bit_set_gen word_size)
+  by (simp add: word_set_nth_iff)
 
 lemma one_bit_shiftl: "set_bit 0 n True = (1 :: 'a :: len word) << n"
   apply (rule word_eqI)
-  apply (auto simp add: test_bit_set_gen nth_shiftl word_size
-              simp del: word_set_bit_0 shiftl_1)
+  apply (auto simp add: word_size bit_simps)
   done
 
-lemmas one_bit_pow = trans [OF one_bit_shiftl shiftl_1]
+lemma one_bit_pow: "set_bit 0 n True = (2 :: 'a :: len word) ^ n"
+  by (simp add: one_bit_shiftl shiftl_def)
 
 end
