lib/Word_Lib/Examples.thy
@@ -5,8 +5,969 @@
  *)
 
 theory Examples
-  imports Bitwise Next_and_Prev Generic_set_bit Word_Syntax Signed_Division_Word
+  imports
+    Bit_Shifts_Infix_Syntax Next_and_Prev Signed_Division_Word Bitwise
 begin
+
+context
+  includes bit_operations_syntax
+begin
+
+section \<open>\<^typ>\<open>nat\<close>\<close>
+
+lemma
+  \<open>bit (1705 :: nat) (Suc (Suc (Suc 0)))\<close>
+  by simp
+
+lemma
+  \<open>bit (1705 :: nat) 3\<close>
+  by simp
+
+lemma
+  \<open>\<not> bit (1 :: nat) (Suc (Suc (Suc 0)))\<close>
+  by simp
+
+lemma
+  \<open>\<not> bit (1 :: nat) 3\<close>
+  by simp
+
+lemma
+  \<open>(1705 :: nat) AND 42 = 40\<close>
+  by simp
+
+lemma
+  \<open>(1705 :: nat) AND Suc 0 = 1\<close>
+  by simp
+
+lemma
+  \<open>(1705 :: nat) OR 42 = 1707\<close>
+  by simp
+
+lemma
+  \<open>(1705 :: nat) OR Suc 0 = 1705\<close>
+  by simp
+
+lemma
+  \<open>(1705 :: nat) XOR 42 = 1667\<close>
+  by simp
+
+lemma
+  \<open>(1705 :: nat) XOR 1 = 1704\<close>
+  by simp
+
+lemma
+  \<open>push_bit 3 (1705 :: nat) = 13640\<close>
+  by simp
+
+lemma
+  \<open>push_bit (Suc (Suc (Suc 0))) (1705 :: nat) = 13640\<close>
+  by simp
+
+lemma
+  \<open>push_bit 3 (Suc 0) = 8\<close>
+  by simp
+
+lemma
+  \<open>push_bit (Suc (Suc (Suc 0))) (Suc 0) = 8\<close>
+  by simp
+
+lemma
+  \<open>(1705 :: nat) << 3 = 13640\<close>
+  by simp
+
+lemma
+  \<open>(1705 :: nat) << Suc (Suc (Suc 0)) = 13640\<close>
+  by simp
+
+lemma
+  \<open>Suc 0 << 3 = 8\<close>
+  by simp
+
+lemma
+  \<open>Suc 0 << Suc (Suc (Suc 0)) = 8\<close>
+  by simp
+
+lemma
+  \<open>drop_bit 3 (1705 :: nat) = 213\<close>
+  by simp
+
+lemma
+  \<open>drop_bit (Suc (Suc (Suc 0))) (1705 :: nat) = 213\<close>
+  by simp
+
+lemma
+  \<open>drop_bit 3 (Suc 0) = 0\<close>
+  by simp
+
+lemma
+  \<open>drop_bit (Suc (Suc (Suc 0))) (Suc 0) = 0\<close>
+  by simp
+
+lemma
+  \<open>(1705 :: nat) >> 3 = 213\<close>
+  by simp
+
+lemma
+  \<open>(1705 :: nat) >> Suc (Suc (Suc 0)) = 213\<close>
+  by simp
+
+lemma
+  \<open>Suc 0 >> 3 = 0\<close>
+  by simp
+
+lemma
+  \<open>Suc 0 >> Suc (Suc (Suc 0)) = 0\<close>
+  by simp
+
+lemma
+  \<open>take_bit 3 (1705 :: nat) = 1\<close>
+  by simp
+
+lemma
+  \<open>take_bit (Suc (Suc (Suc 0))) (1705 :: nat) = 1\<close>
+  by (simp flip: add_2_eq_Suc)
+
+lemma
+  \<open>take_bit 3 (Suc 0) = 1\<close>
+  by simp
+
+lemma
+  \<open>take_bit (Suc (Suc (Suc 0))) (Suc 0) = 1\<close>
+  by simp
+
+
+section \<open>\<^typ>\<open>int\<close>\<close>
+
+lemma
+  \<open>bit (1705 :: int) (Suc (Suc (Suc 0)))\<close>
+  by simp
+
+lemma
+  \<open>bit (1705 :: int) 3\<close>
+  by simp
+
+lemma
+  \<open>\<not> bit (- 1705 :: int) (Suc (Suc (Suc 0)))\<close>
+  by simp
+
+lemma
+  \<open>\<not> bit (- 1705 :: int) 3\<close>
+  by simp
+
+lemma
+  \<open>\<not> bit (1 :: int) (Suc (Suc (Suc 0)))\<close>
+  by simp
+
+lemma
+  \<open>\<not> bit (1 :: int) 3\<close>
+  by simp
+
+lemma
+  \<open>(NOT 1705 :: int) = - 1706\<close>
+  by simp
+
+lemma
+  \<open>(NOT (- 42 :: int)) = 41\<close>
+  by simp
+
+lemma
+  \<open>(NOT 1 :: int) = - 2\<close>
+  by simp
+
+lemma
+  \<open>(1705 :: int) AND 42 = 40\<close>
+  by simp
+
+lemma
+  \<open>(1705 :: int) AND - 42 = 1664\<close>
+  by simp
+
+lemma
+  \<open>(1705 :: int) AND 1 = 1\<close>
+  by simp
+
+lemma
+  \<open>- (1705 :: int) AND 42 = 2\<close>
+  by simp
+
+lemma
+  \<open>- (1705 :: int) AND - 42 = - 1706\<close>
+  by simp
+
+lemma
+  \<open>- (1705 :: int) AND 1 = 1\<close>
+  by simp
+
+lemma
+  \<open>(1705 :: int) OR 42 = 1707\<close>
+  by simp
+
+lemma
+  \<open>(1705 :: int) OR - 42 = - 1\<close>
+  by simp
+
+lemma
+  \<open>(1705 :: int) OR 1 = 1705\<close>
+  by simp
+
+lemma
+  \<open>- (1705 :: int) OR 42 = - 1665\<close>
+  by simp
+
+lemma
+  \<open>- (1705 :: int) OR - 42 = - 41\<close>
+  by simp
+
+lemma
+  \<open>- (1705 :: int) OR 1 = - 1705\<close>
+  by simp
+
+lemma
+  \<open>(1705 :: int) XOR 42 = 1667\<close>
+  by simp
+
+lemma
+  \<open>(1705 :: int) XOR - 42 = - 1665\<close>
+  by simp
+
+lemma
+  \<open>(1705 :: int) XOR 1 = 1704\<close>
+  by simp
+
+lemma
+  \<open>- (1705 :: int) XOR 42 = - 1667\<close>
+  by simp
+
+lemma
+  \<open>- (1705 :: int) XOR - 42 = 1665\<close>
+  by simp
+
+lemma
+  \<open>- (1705 :: int) XOR 1 = - 1706\<close>
+  by simp
+
+lemma
+  \<open>push_bit 3 (1705 :: int) = 13640\<close>
+  by simp
+
+lemma
+  \<open>push_bit (Suc (Suc (Suc 0))) (1705 :: int) = 13640\<close>
+  by simp
+
+lemma
+  \<open>push_bit 3 (- 1705 :: int) = - 13640\<close>
+  by simp
+
+lemma
+  \<open>push_bit (Suc (Suc (Suc 0))) (- 1705 :: int) = - 13640\<close>
+  by simp
+
+lemma
+  \<open>push_bit 3 (1 :: int) = 8\<close>
+  by simp
+
+lemma
+  \<open>push_bit (Suc (Suc (Suc 0))) (1 :: int) = 8\<close>
+  by simp
+
+lemma
+  \<open>push_bit 3 (- 1 :: int) = - 8\<close>
+  by (simp add: mask_eq_exp_minus_1)
+
+lemma
+  \<open>push_bit (Suc (Suc (Suc 0))) (- 1 :: int) = - 8\<close>
+  by (simp add: mask_eq_exp_minus_1)
+
+lemma
+  \<open>(1705 :: int) << 3  = 13640\<close>
+  by simp
+
+lemma
+  \<open>(1705 :: int) << Suc (Suc (Suc 0)) = 13640\<close>
+  by simp
+
+lemma
+  \<open>(- 1705 :: int) << 3 = - 13640\<close>
+  by simp
+
+lemma
+  \<open>(- 1705 :: int) << Suc (Suc (Suc 0)) = - 13640\<close>
+  by simp
+
+lemma
+  \<open>(1 :: int) << 3 = 8\<close>
+  by simp
+
+lemma
+  \<open>(1 :: int) << Suc (Suc (Suc 0)) = 8\<close>
+  by simp
+
+lemma
+  \<open>(- 1 :: int) << 3 = - 8\<close>
+  by (simp add: mask_eq_exp_minus_1)
+
+lemma
+  \<open>(- 1 :: int) << Suc (Suc (Suc 0)) = - 8\<close>
+  by simp
+
+lemma
+  \<open>drop_bit 3 (1705 :: int) = 213\<close>
+  by simp
+
+lemma
+  \<open>drop_bit (Suc (Suc (Suc 0))) (1705 :: int) = 213\<close>
+  by simp
+
+lemma
+  \<open>drop_bit 3 (- 1705 :: int) = - 214\<close>
+  by simp
+
+lemma
+  \<open>drop_bit (Suc (Suc (Suc 0))) (- 1705 :: int) = - 214\<close>
+  by simp
+
+lemma
+  \<open>drop_bit 3 (1 :: int) = 0\<close>
+  by simp
+
+lemma
+  \<open>drop_bit (Suc (Suc (Suc 0))) (1 :: int) = 0\<close>
+  by simp
+
+lemma
+  \<open>(1705 :: int) >> 3 = 213\<close>
+  by simp
+
+lemma
+  \<open>(1705 :: int) >> Suc (Suc (Suc 0)) = 213\<close>
+  by simp
+
+lemma
+  \<open>(- 1705 :: int) >> 3 = - 214\<close>
+  by simp
+
+lemma
+  \<open>(- 1705 :: int) >> Suc (Suc (Suc 0)) = - 214\<close>
+  by simp
+
+lemma
+  \<open>(1 :: int) >> 3 = 0\<close>
+  by simp
+
+lemma
+  \<open>(1 :: int) >> Suc (Suc (Suc 0)) = 0\<close>
+  by simp
+
+lemma
+  \<open>take_bit 3 (1705 :: int) = 1\<close>
+  by simp
+
+lemma
+  \<open>take_bit (Suc (Suc (Suc 0))) (1705 :: int) = 1\<close>
+  by (simp flip: add_2_eq_Suc)
+
+lemma
+  \<open>take_bit 3 (- 1705 :: int) = 7\<close>
+  by simp
+
+lemma
+  \<open>take_bit (Suc (Suc (Suc 0))) (- 1705 :: int) = 7\<close>
+  by (simp flip: add_2_eq_Suc)
+
+lemma
+  \<open>take_bit 3 (1 :: int) = 1\<close>
+  by simp
+
+lemma
+  \<open>take_bit (Suc (Suc (Suc 0))) (1 :: int) = 1\<close>
+  by simp
+
+lemma
+  \<open>take_bit 3 (- 1 :: int) = 7\<close>
+  by (simp add: mask_eq_exp_minus_1)
+
+lemma
+  \<open>take_bit (Suc (Suc (Suc 0))) (- 1 :: int) = 7\<close>
+  by (simp add: mask_eq_exp_minus_1)
+
+lemma
+  \<open>signed_take_bit 3 (1705 :: int) = - 7\<close>
+  by simp
+
+lemma
+  \<open>signed_take_bit (Suc (Suc (Suc 0))) (1705 :: int) = - 7\<close>
+  by simp
+
+lemma
+  \<open>signed_take_bit 3 (- 1705 :: int) = 7\<close>
+  by simp
+
+lemma
+  \<open>signed_take_bit (Suc (Suc (Suc 0))) (- 1705 :: int) = 7\<close>
+  by simp
+
+lemma
+  \<open>signed_take_bit 3 (1 :: int) = 1\<close>
+  by simp
+
+lemma
+  \<open>signed_take_bit (Suc (Suc (Suc 0))) (1 :: int) = 1\<close>
+  by simp
+
+
+section \<open>\<^typ>\<open>'a word\<close>\<close>
+
+lemma
+  \<open>(1705 :: 8 word) = 169\<close>
+  by simp
+
+lemma
+  \<open>(- 1705 :: 8 word) = 87\<close>
+  by simp
+
+lemma
+  \<open>(257 :: 8 word) = 1\<close>
+  by simp
+
+lemma
+  \<open>(42 :: 8 word) \<le> 1705\<close>
+  by simp
+
+lemma
+  \<open>(- 42 :: 8 word) \<le> 230\<close>
+  by simp
+
+lemma
+  \<open>(42 :: 8 word) \<le> - 1705\<close>
+  by simp
+
+lemma
+  \<open>- (42 :: 8 word) \<le> 235\<close>
+  by simp
+
+lemma
+  \<open>(1 :: 8 word) \<le> 1705\<close>
+  by simp
+
+lemma
+  \<open>(- 1 :: 8 word) \<le> 65535\<close>
+  by simp
+
+lemma
+  \<open>(42 :: 8 word) < 1705\<close>
+  by simp
+
+lemma
+  \<open>(- 42 :: 8 word) < 230\<close>
+  by simp
+
+lemma
+  \<open>(42 :: 8 word) < - 1705\<close>
+  by simp
+
+lemma
+  \<open>- (42 :: 8 word) < 230\<close>
+  by simp
+
+lemma
+  \<open>(1 :: 8 word) < 1705\<close>
+  by simp
+
+lemma
+  \<open>(1705 :: 8 word) < - 1\<close>
+  by simp
+
+lemma
+  \<open>(42 :: 8 word) \<le>s 1333\<close>
+  by simp
+
+lemma
+  \<open>(- 42 :: 8 word) \<le>s 230\<close>
+  by simp
+
+lemma
+  \<open>(42 :: 8 word) \<le>s - 1705\<close>
+  by simp
+
+lemma
+  \<open>- (42 :: 8 word) \<le>s - 1705\<close>
+  by simp
+
+lemma
+  \<open>(1 :: 8 word) \<le>s 42\<close>
+  by simp
+
+lemma
+  \<open>(42 :: 8 word) <s 1333\<close>
+  by simp
+
+lemma
+  \<open>(- 42 :: 8 word) <s 230\<close>
+  by simp
+
+lemma
+  \<open>(42 :: 8 word) <s - 1705\<close>
+  by simp
+
+lemma
+  \<open>- (42 :: 8 word) <s - 1705\<close>
+  by simp
+
+lemma
+  \<open>(1 :: 8 word) <s 42\<close>
+  by simp
+
+lemma
+  \<open>bit (1705 :: 16 word) (Suc (Suc (Suc 0)))\<close>
+  by simp
+
+lemma
+  \<open>bit (1705 :: 16 word) 3\<close>
+  by simp
+
+lemma
+  \<open>\<not> bit (- 1705 :: 16 word) (Suc (Suc (Suc 0)))\<close>
+  by simp
+
+lemma
+  \<open>\<not> bit (- 1705 :: 16 word) 3\<close>
+  by simp
+
+lemma
+  \<open>\<not> bit (1 :: 'a::len word) (Suc (Suc (Suc 0)))\<close>
+  by simp
+
+lemma
+  \<open>\<not> bit (1 :: 'a::len word) 3\<close>
+  by simp
+
+lemma
+  \<open>(NOT 1705 :: 'a::len word) = - 1706\<close>
+  by simp
+
+lemma
+  \<open>(NOT (- 42 :: 'a::len word)) = 41\<close>
+  by simp
+
+lemma
+  \<open>(NOT 1 :: 'a::len word) = - 2\<close>
+  by simp
+
+lemma
+  \<open>(1705 :: 'a::len word) AND 42 = 40\<close>
+  by simp
+
+lemma
+  \<open>(1705 :: 'a::len word) AND - 42 = 1664\<close>
+  by simp
+
+lemma
+  \<open>(1705 :: 'a::len word) AND 1 = 1\<close>
+  by simp
+
+lemma
+  \<open>- (1705 :: 'a::len word) AND 42 = 2\<close>
+  by simp
+
+lemma
+  \<open>- (1705 :: 'a::len word) AND - 42 = - 1706\<close>
+  by simp
+
+lemma
+  \<open>- (1705 :: 'a::len word) AND 1 = 1\<close>
+  by simp
+
+lemma
+  \<open>(1705 :: 'a::len word) OR 42 = 1707\<close>
+  by simp
+
+lemma
+  \<open>(1705 :: 'a::len word) OR - 42 = - 1\<close>
+  by simp
+
+lemma
+  \<open>(1705 :: 'a::len word) OR 1 = 1705\<close>
+  by simp
+
+lemma
+  \<open>- (1705 :: 'a::len word) OR 42 = - 1665\<close>
+  by simp
+
+lemma
+  \<open>- (1705 :: 'a::len word) OR - 42 = - 41\<close>
+  by simp
+
+lemma
+  \<open>- (1705 :: 'a::len word) OR 1 = - 1705\<close>
+  by simp
+
+lemma
+  \<open>(1705 :: 'a::len word) XOR 42 = 1667\<close>
+  by simp
+
+lemma
+  \<open>(1705 :: 'a::len word) XOR - 42 = - 1665\<close>
+  by simp
+
+lemma
+  \<open>(1705 :: 'a::len word) XOR 1 = 1704\<close>
+  by simp
+
+lemma
+  \<open>- (1705 :: 'a::len word) XOR 42 = - 1667\<close>
+  by simp
+
+lemma
+  \<open>- (1705 :: 'a::len word) XOR - 42 = 1665\<close>
+  by simp
+
+lemma
+  \<open>- (1705 :: 'a::len word) XOR 1 = - 1706\<close>
+  by simp
+
+lemma
+  \<open>push_bit 3 (1705 :: 'a::len word) = 13640\<close>
+  by simp
+
+lemma
+  \<open>push_bit (Suc (Suc (Suc 0))) (1705 :: 'a::len word) = 13640\<close>
+  by simp
+
+lemma
+  \<open>push_bit 3 (- 1705 :: 'a::len word) = - 13640\<close>
+  by simp
+
+lemma
+  \<open>push_bit (Suc (Suc (Suc 0))) (- 1705 :: 'a::len word) = - 13640\<close>
+  by simp
+
+lemma
+  \<open>push_bit 3 (1 :: 'a::len word) = 8\<close>
+  by simp
+
+lemma
+  \<open>push_bit (Suc (Suc (Suc 0))) (1 :: 'a::len word) = 8\<close>
+  by simp
+
+lemma
+  \<open>push_bit 3 (- 1 :: 'a::len word) = - 8\<close>
+  by (simp add: mask_eq_exp_minus_1)
+
+lemma
+  \<open>push_bit (Suc (Suc (Suc 0))) (- 1 :: 'a::len word) = - 8\<close>
+  by (simp add: mask_eq_exp_minus_1)
+
+lemma
+  \<open>(1705 :: 'a::len word) << 3 = 13640\<close>
+  by simp
+
+lemma
+  \<open>(1705 :: 'a::len word) << Suc (Suc (Suc 0)) = 13640\<close>
+  by simp
+
+lemma
+  \<open>(- 1705 :: 'a::len word) << 3 = - 13640\<close>
+  by simp
+
+lemma
+  \<open>(- 1705 :: 'a::len word) << Suc (Suc (Suc 0)) = - 13640\<close>
+  by simp
+
+lemma
+  \<open>(1 :: 'a::len word) << 3 = 8\<close>
+  by simp
+
+lemma
+  \<open>(1 :: 'a::len word) << Suc (Suc (Suc 0)) = 8\<close>
+  by simp
+
+lemma
+  \<open>(- 1 :: 'a::len word) << 3 = - 8\<close>
+  by (simp add: mask_eq_exp_minus_1)
+
+lemma
+  \<open>(- 1 :: 'a::len word) << Suc (Suc (Suc 0)) = - 8\<close>
+  by simp
+
+lemma
+  \<open>drop_bit 3 (1705 :: 16 word) = 213\<close>
+  by simp
+
+lemma
+  \<open>drop_bit (Suc (Suc (Suc 0))) (1705 :: 16 word) = 213\<close>
+  by simp
+
+lemma
+  \<open>drop_bit 3 (- 1705 :: 16 word) = 7978\<close>
+  by simp
+
+lemma
+  \<open>drop_bit (Suc (Suc (Suc 0))) (- 1705 :: 16 word) = 7978\<close>
+  by simp
+
+lemma
+  \<open>drop_bit 3 (1 :: 16 word) = 0\<close>
+  by simp
+
+lemma
+  \<open>drop_bit (Suc (Suc (Suc 0))) (1 :: 16 word) = 0\<close>
+  by simp
+
+lemma
+  \<open>(1705 :: 16 word) >> 3 = 213\<close>
+  by simp
+
+lemma
+  \<open>(1705 :: 16 word) >> Suc (Suc (Suc 0)) = 213\<close>
+  by simp
+
+lemma
+  \<open>(- 1705 :: 16 word) >> 3 = 7978\<close>
+  by simp
+
+lemma
+  \<open>(- 1705 :: 16 word) >> Suc (Suc (Suc 0)) = 7978\<close>
+  by simp
+
+lemma
+  \<open>(1 :: 16 word) >> 3 = 0\<close>
+  by simp
+
+lemma
+  \<open>(1 :: 16 word) >> Suc (Suc (Suc 0)) = 0\<close>
+  by simp
+
+lemma
+  \<open>signed_drop_bit 3 (1705 :: 16 word) = 213\<close>
+  by simp
+
+lemma
+  \<open>signed_drop_bit (Suc (Suc (Suc 0))) (1705 :: 16 word) = 213\<close>
+  by simp
+
+lemma
+  \<open>signed_drop_bit 3 (- 1705 :: 16 word) = - 214\<close>
+  by simp
+
+lemma
+  \<open>signed_drop_bit (Suc (Suc (Suc 0))) (- 1705 :: 16 word) = - 214\<close>
+  by simp
+
+lemma
+  \<open>signed_drop_bit 3 (1 :: 16 word) = 0\<close>
+  by simp
+
+lemma
+  \<open>signed_drop_bit (Suc (Suc (Suc 0))) (1 :: 16 word) = 0\<close>
+  by simp
+
+lemma
+  \<open>(1705 :: 16 word) >>> 3 = 213\<close>
+  by simp
+
+lemma
+  \<open>(1705 :: 16 word) >>> Suc (Suc (Suc 0)) = 213\<close>
+  by simp
+
+lemma
+  \<open>(- 1705 :: 16 word) >>> 3 = - 214\<close>
+  by simp
+
+lemma
+  \<open>(- 1705 :: 16 word) >>> Suc (Suc (Suc 0)) = - 214\<close>
+  by simp
+
+lemma
+  \<open>(1 :: 16 word) >>> 3 = 0\<close>
+  by simp
+
+lemma
+  \<open>(1 :: 16 word) >>> Suc (Suc (Suc 0)) = 0\<close>
+  by simp
+
+lemma
+  \<open>take_bit 3 (1705 :: 16 word) = 1\<close>
+  by simp
+
+lemma
+  \<open>take_bit (Suc (Suc (Suc 0))) (1705 :: 16 word) = 1\<close>
+  by (simp flip: add_2_eq_Suc)
+
+lemma
+  \<open>take_bit 3 (- 1705 :: 16 word) = 7\<close>
+  by simp
+
+lemma
+  \<open>take_bit (Suc (Suc (Suc 0))) (- 1705 :: 16 word) = 7\<close>
+  by (simp flip: add_2_eq_Suc)
+
+lemma
+  \<open>take_bit 3 (1 :: 16 word) = 1\<close>
+  by simp
+
+lemma
+  \<open>take_bit (Suc (Suc (Suc 0))) (1 :: 16 word) = 1\<close>
+  by simp
+
+lemma
+  \<open>take_bit 3 (- 1 :: 16 word) = 7\<close>
+  by (simp add: mask_eq_exp_minus_1)
+
+lemma
+  \<open>take_bit (Suc (Suc (Suc 0))) (- 1 :: 16 word) = 7\<close>
+  by (simp add: mask_eq_exp_minus_1)
+
+lemma
+  \<open>signed_take_bit 3 (1705 :: 16 word) = - 7\<close>
+  by simp
+
+lemma
+  \<open>signed_take_bit (Suc (Suc (Suc 0))) (1705 :: 16 word) = - 7\<close>
+  by simp
+
+lemma
+  \<open>signed_take_bit 3 (- 1705 :: 16 word) = 7\<close>
+  by simp
+
+lemma
+  \<open>signed_take_bit (Suc (Suc (Suc 0))) (- 1705 :: 16 word) = 7\<close>
+  by simp
+
+lemma
+  \<open>signed_take_bit 3 (1 :: 16 word) = 1\<close>
+  by simp
+
+lemma
+  \<open>signed_take_bit (Suc (Suc (Suc 0))) (1 :: 16 word) = 1\<close>
+  by simp
+
+lemma
+  \<open>(1705 :: 16 word) div 42 = 40\<close>
+  by simp
+
+lemma
+  \<open>(- 1705 :: 16 word) div 42 = 1519\<close>
+  by simp
+
+lemma
+  \<open>(1705 :: 16 word) div - 42 = 0\<close>
+  by simp
+
+lemma
+  \<open>(- 1705 :: 16 word) div - 42 = 0\<close>
+  by simp
+
+lemma
+  \<open>(1705 :: 16 word) div 1 = 1705\<close>
+  by simp
+
+lemma
+  \<open>(1705 :: 16 word) div - 1 = 0\<close>
+  by simp
+
+lemma
+  \<open>(1 :: 16 word) div 42 = 0\<close>
+  by simp
+
+lemma
+  \<open>(- 1 :: 16 word) div 42 = 1560\<close>
+  by simp
+
+lemma
+  \<open>(1705 :: 16 word) mod 42 = 25\<close>
+  by simp
+
+lemma
+  \<open>(- 1705 :: 16 word) mod 42 = 33\<close>
+  by simp
+
+lemma
+  \<open>(1705 :: 16 word) mod - 42 = 1705\<close>
+  by simp
+
+lemma
+  \<open>(- 1705 :: 16 word) mod - 42 = 63831\<close>
+  by simp
+
+lemma
+  \<open>(1705 :: 16 word) mod 1 = 0\<close>
+  by simp
+
+lemma
+  \<open>(1705 :: 16 word) mod - 1 = 1705\<close>
+  by simp
+
+lemma
+  \<open>(1 :: 16 word) mod 42 = 1\<close>
+  by simp
+
+lemma
+  \<open>(- 1 :: 16 word) mod 42 = 15\<close>
+  by simp
+
+lemma
+  \<open>(1705 :: 16 word) sdiv 42 = 40\<close>
+  by simp
+
+lemma
+  \<open>(- 1705 :: 16 word) sdiv 42 = 65496\<close>
+  by simp
+
+lemma
+  \<open>(1705 :: 16 word) sdiv - 42 = 65496\<close>
+  by simp
+
+lemma
+  \<open>(- 1705 :: 16 word) sdiv - 42 = 40\<close>
+  by simp
+
+lemma
+  \<open>(1705 :: 16 word) sdiv 1 = 1705\<close>
+  by simp
+
+lemma
+  \<open>(1705 :: 16 word) sdiv - 1 = 63831\<close>
+  by simp
+
+lemma
+  \<open>(1 :: 16 word) sdiv 42 = 0\<close>
+  by simp
+
+lemma
+  \<open>(- 1 :: 16 word) sdiv 42 = 0\<close>
+  by simp
+
+lemma
+  \<open>(1705 :: 16 word) smod 42 = 25\<close>
+  by simp
+
+lemma
+  \<open>(- 1705 :: 16 word) smod 42 = 65511\<close>
+  by simp
+
+lemma
+  \<open>(1705 :: 16 word) smod - 42 = 25\<close>
+  by simp
+
+lemma
+  \<open>(- 1705 :: 16 word) smod - 42 = 65511\<close>
+  by simp
+
+lemma
+  \<open>(1705 :: 16 word) smod 1 = 0\<close>
+  by simp
+
+lemma
+  \<open>(1705 :: 16 word) smod - 1 = 0\<close>
+  by simp
+
+lemma
+  \<open>(1 :: 16 word) smod 42 = 1\<close>
+  by simp
+
+lemma
+  \<open>(- 1 :: 16 word) smod 42 = 65535\<close>
+  by simp
 
 text "modulus"
 
@@ -68,15 +1029,6 @@ lemma "i < x \<Longrightarrow> i < i + 1" for i x :: "'a::len word"
 lemma "i < x \<Longrightarrow> i < i + 1" for i x :: "'a::len word"
   by unat_arith
 
-text "bool lists"
-
-lemma "of_bl [True, False, True, True] = (0b1011::'a::len word)" by simp
-
-lemma "to_bl (0b110::4 word) = [False, True, True, False]" by simp
-
-lemma "of_bl (replicate 32 True) = (0xFFFFFFFF::32 word)"
-  by (simp add: numeral_eq_Suc)
-
 text "bit operations"
 
 lemma "0b110 AND 0b101 = (0b100 :: 32 word)" by simp
@@ -96,13 +1048,13 @@ lemma "NOT 0 = (255 :: 8 word)" by simp
 
 lemma "(-1 :: 32 word) = 0xFFFFFFFF" by simp
 
-lemma "(0b0010 :: 4 word) !! 1" by simp
-lemma "\<not> (0b0010 :: 4 word) !! 0" by simp
-lemma "\<not> (0b1000 :: 3 word) !! 4" by simp
-lemma "\<not> (1 :: 3 word) !! 2" by simp
+lemma "bit (0b0010 :: 4 word) 1" by simp
+lemma "\<not> bit (0b0010 :: 4 word) 0" by simp
+lemma "\<not> bit (0b1000 :: 3 word) 4" by simp
+lemma "\<not> bit (1 :: 3 word) 2" by simp
 
-lemma "(0b11000 :: 10 word) !! n = (n = 4 \<or> n = 3)"
-  by (auto simp add: bin_nth_Bit0 bin_nth_Bit1)
+lemma "bit (0b11000 :: 10 word) n = (n = 4 \<or> n = 3)"
+  by (auto simp add: bit_numeral_rec bit_1_iff split: nat.splits)
 
 lemma "set_bit 55 7 True = (183::'a::len word)" by simp
 lemma "set_bit 0b0010 7 True = (0b10000010::'a::len word)" by simp
@@ -122,7 +1074,8 @@ lemma   "msb (0b1000::4 word)" by simp
 lemma "\<not> msb (1::4 word)" by simp
 lemma "\<not> msb (0::4 word)" by simp
 
-lemma "word_cat (27::4 word) (27::8 word) = (2843::'a::len word)" by simp
+lemma "word_cat (27::4 word) (27::8 word) = (2843::'a::len word)"
+  by simp
 lemma "word_cat (0b0011::4 word) (0b1111::6word) = (0b0011001111 :: 10 word)"
   by simp
 
@@ -158,6 +1111,43 @@ lemma "word_next (2:: 8 word) = 3" by eval
 lemma "word_next (255:: 8 word) = 255" by eval
 lemma "word_prev (2:: 8 word) = 1" by eval
 lemma "word_prev (0:: 8 word) = 0" by eval
+
+text \<open>singed division\<close>
+
+lemma
+  "( 4 :: 32 word) sdiv  4 =  1"
+  "(-4 :: 32 word) sdiv  4 = -1"
+  "(-3 :: 32 word) sdiv  4 =  0"
+  "( 3 :: 32 word) sdiv -4 =  0"
+  "(-3 :: 32 word) sdiv -4 =  0"
+  "(-5 :: 32 word) sdiv -4 =  1"
+  "( 5 :: 32 word) sdiv -4 = -1"
+  by (simp_all add: sdiv_word_def signed_divide_int_def)
+
+lemma
+  "( 4 :: 32 word) smod  4 =   0"
+  "( 3 :: 32 word) smod  4 =   3"
+  "(-3 :: 32 word) smod  4 =  -3"
+  "( 3 :: 32 word) smod -4 =   3"
+  "(-3 :: 32 word) smod -4 =  -3"
+  "(-5 :: 32 word) smod -4 =  -1"
+  "( 5 :: 32 word) smod -4 =   1"
+  by (simp_all add: smod_word_def signed_modulo_int_def signed_divide_int_def)
+
+
+text \<open>comparison\<close>
+
+lemma "1 < (1024::32 word) \<and> 1 \<le> (1024::32 word)"
+  by simp
+
+text "bool lists"
+
+lemma "of_bl [True, False, True, True] = (0b1011::'a::len word)" by simp
+
+lemma "to_bl (0b110::4 word) = [False, True, True, False]" by simp
+
+lemma "of_bl (replicate 32 True) = (0xFFFFFFFF::32 word)"
+  by (simp add: numeral_eq_Suc)
 
 text "proofs using bitwise expansion"
 
@@ -199,28 +1189,6 @@ lemma shiftr_overflow: "32 \<le> a \<Longrightarrow> b >> a = 0"
 lemma "((x :: 32 word) >> 3) AND 7 = (x AND 56) >> 3"
   by word_bitwise
 
-(* Tests *)
-lemma
-  "( 4 :: 32 word) sdiv  4 =  1"
-  "(-4 :: 32 word) sdiv  4 = -1"
-  "(-3 :: 32 word) sdiv  4 =  0"
-  "( 3 :: 32 word) sdiv -4 =  0"
-  "(-3 :: 32 word) sdiv -4 =  0"
-  "(-5 :: 32 word) sdiv -4 =  1"
-  "( 5 :: 32 word) sdiv -4 = -1"
-  by (simp_all add: sdiv_word_def signed_divide_int_def)
-
-lemma
-  "( 4 :: 32 word) smod  4 =   0"
-  "( 3 :: 32 word) smod  4 =   3"
-  "(-3 :: 32 word) smod  4 =  -3"
-  "( 3 :: 32 word) smod -4 =   3"
-  "(-3 :: 32 word) smod -4 =  -3"
-  "(-5 :: 32 word) smod -4 =  -1"
-  "( 5 :: 32 word) smod -4 =   1"
-  by (simp_all add: smod_word_def signed_modulo_int_def signed_divide_int_def)
-
-lemma "1 < (1024::32 word) \<and> 1 \<le> (1024::32 word)"
-  by simp
+end
 
 end
