lib/Word_Lib/Signed_Words.thy
@@ -81,7 +81,7 @@ lemma word_le_ucast_sless:
   apply simp_all
   apply transfer
   apply (simp add: signed_take_bit_take_bit)
-  apply (metis add.commute mask_eq_exp_minus_1 mask_eq_take_bit_minus_one take_bit_incr_eq zle_add1_eq_le)
+  apply (metis add.commute mask_eq_exp_minus_1 take_bit_incr_eq zle_add1_eq_le)
   done
 
 lemma zero_sle_ucast:
@@ -92,6 +92,21 @@ lemma zero_sle_ucast:
    apply (simp_all add: take_bit_Suc_from_most bit_simps)
   apply (simp_all add: bit_simps disjunctive_add)
   done
+
+lemma nth_w2p_scast:
+  "(bit (scast ((2::'a::len signed word) ^ n) :: 'a word) m)
+         \<longleftrightarrow> (bit (((2::'a::len  word) ^ n) :: 'a word) m)"
+  by (simp add: bit_simps)
+
+lemma scast_nop1 [simp]:
+  "((scast ((of_int x)::('a::len) word))::'a signed word) = of_int x"
+  by transfer (simp add: take_bit_signed_take_bit)
+
+lemma scast_nop2 [simp]:
+  "((scast ((of_int x)::('a::len) signed word))::'a word) = of_int x"
+  by transfer (simp add: take_bit_signed_take_bit)
+
+lemmas scast_nop = scast_nop1 scast_nop2 scast_id
 
 type_synonym 'a sword = "'a signed word"
 
